Accumulative state monad for wlocal_ctx in codegen

theories/compiler/codegen.v
@@ -12,6 +12,7 @@ From ExtLib.Structures Require Import Monoid Monads.
 From Wasm Require datatypes.
 
 Require Import RichWasm.compiler.prelude.
+Require Import RichWasm.compiler.accum.
 Require Import RichWasm.util.
 
 Module W := Wasm.datatypes.
@@ -19,7 +20,7 @@ Module W := Wasm.datatypes.
 Notation wlocal_ctx := (list W.value_type) (only parsing).
 
 Record codegen (A : Type) :=
-  { uncodegen : stateT wlocal_ctx
+  { uncodegen : accumT W.value_type
                        (writerT (@Monoid_list_app W.basic_instruction)
                                 (sum error))
                        A }.
@@ -37,24 +38,26 @@ Global Instance MonadExc_codegen : MonadExc error codegen :=
   { raise := fun _ => Build_codegen ∘ raise;
     catch := fun _ b h => Build_codegen (catch (uncodegen b) (uncodegen ∘ h)) }.
 
-Global Instance MonadState_codegen : MonadState wlocal_ctx codegen :=
-  { get := Build_codegen get;
-    put := Build_codegen ∘ put }.
+Definition get : codegen (list W.value_type) :=
+  Build_codegen (mkAccumT (fun s => ret (s, nil))).
+
+Definition acc (s' : list W.value_type) : codegen () :=
+  Build_codegen (mkAccumT (fun s => ret (tt, s'))).
 
 Global Instance MonadWriter_codegen : MonadWriter (@Monoid_list_app W.basic_instruction) codegen :=
   { tell := Build_codegen ∘ tell;
     listen := fun _ => Build_codegen ∘ listen ∘ uncodegen;
     (* Work around broken implementation of `pass` in ExtLib.
        https://github.com/rocq-community/coq-ext-lib/issues/153 *)
-    pass := fun _ c => Build_codegen (mkStateT (fun s =>
-      pass ('(x, f, s) ← runStateT (uncodegen c) s;
-            ret (x, s, f)))) }.
+    pass := fun _ c => Build_codegen (mkAccumT (fun s =>
+      pass ('(x, f, s') ← runAccumT (uncodegen c) s;
+            ret (x, s', f)))) }.
 
 Definition lift_error {A : Type} (c : error + A) : codegen A :=
   Build_codegen (lift (lift c)).
 
 Definition run_codegen {A : Type} (c : codegen A) (wl : wlocal_ctx) : error + A * wlocal_ctx * W.expr :=
-  match runWriterT (runStateT (uncodegen c) wl) with
+  match runWriterT (runAccumT (uncodegen c) wl) with
   | inl e => inl e
   | inr x => inr (PPair.pfst x, PPair.psnd x)
   end.
@@ -87,7 +90,7 @@ Lemma runWriterT_sum_bind_dist {A B L E}
   (c : writerT m (sum E) A)
   (f : A -> writerT m (sum E) B)
   (x : B)
-  (l l1 : L) :
+  (l : L) :
   runWriterT (c ≫= f) = inr (PPair.ppair x l) ->
   exists x1 l1 l2,
   runWriterT c = inr (PPair.ppair x1 l1) /\
@@ -112,78 +115,94 @@ Proof.
   - congruence.
 Qed.
 
-Lemma runWriterT_runStateT_sum_bind_dist {E L S A B}
+Lemma runWriterT_runAccumT_sum_bind_dist {E L S A B}
   (m : Monoid L)
-  (c : stateT S (writerT m (sum E)) A)
-  (f : A -> stateT S (writerT m (sum E)) B)
-  (s s' : S)
+  (mL : MonoidLaws m)
+  (c : accumT S (writerT m (sum E)) A)
+  (f : A -> accumT S (writerT m (sum E)) B)
+  (s s' : list S)
   (l : L)
   (x : B) :
-  runWriterT (runStateT (c ≫= f) s) = inr (PPair.ppair (x, s') l) ->
-  exists x1 s1 l1 l2,
-  runWriterT (runStateT c s) = inr (PPair.ppair (x1, s1) l1) /\
-  runWriterT (runStateT (f x1) s1) = inr (PPair.ppair (x, s') l2) /\
+  runWriterT (runAccumT (c ≫= f) s) = inr (PPair.ppair (x, s') l) ->
+  exists x1 s1 s2 l1 l2,
+  runWriterT (runAccumT c s) = inr (PPair.ppair (x1, s1) l1) /\
+  runWriterT (runAccumT (f x1) (s ++ s1)) = inr (PPair.ppair (x, s2) l2) /\
+  s' = s1 ++ s2 /\
   l = m.(monoid_plus) l1 l2.
 Proof.
   intros H.
   unfold mbind, MBind_Monad, runStateT, flip, bind, Monad_stateT in H.
   apply runWriterT_sum_bind_dist in H.
-  destruct H as (x1 & l1 & l2 & H1 & H2 & H3).
-  - destruct x1 as [x1 s1].
-    exists x1.
-    exists s1.
-    exists l1.
-    exists l2.
-    split; first assumption.
-    split; assumption.
-  - apply l.
+  destruct H as ([x1 s1] & l1 & l2 & H1 & H2 & H3).
+  apply runWriterT_sum_bind_dist in H2.
+  destruct H2 as ([x2 s2] & l3 & l4 & ? & ? & ?).
+  exists x1, s1, s2, l1, l2.
+  split; first assumption.
+  cbn in *.
+  inversion H0; subst.
+  split; [|split].
+  - rewrite H.
+    by rewrite monoid_runit.
+  - auto.
+  - auto.
 Qed.
 
 Lemma run_codegen_def {A} (c : codegen A) wl wl' x es:
   run_codegen c wl = inr (x, wl', es) <->
-  runWriterT (runStateT (uncodegen c) wl) = inr (PPair.ppair (x, wl') es).
+  runWriterT (runAccumT (uncodegen c) wl) = inr (PPair.ppair (x, wl') es).
 Proof.
   split.
   {
     intros H.
     unfold run_codegen in H.
-    destruct (runWriterT (runStateT (uncodegen c) wl)); first congruence.
+    destruct (runWriterT (runAccumT (uncodegen c) wl)); first congruence.
     inversion H.
     reflexivity.
   }
   {
     intros H.
     unfold run_codegen.
-    destruct (runWriterT (runStateT (uncodegen c) wl)); first congruence.
+    destruct (runWriterT (runAccumT (uncodegen c) wl)); first congruence.
     inversion H.
     reflexivity.
   }
 Qed.
 
+Global Instance MonoidLaws_list {T} : MonoidLaws (@Monoid_list_app T).
+Proof.
+  split.
+  - intros xs ys zs.
+    symmetry. apply app_assoc.
+  - intros xs.
+    apply eq_refl.
+  - intros xs.
+    apply app_nil_r.
+Qed.
+
 Lemma run_codegen_bind_dist {A B} (c : codegen A) (f : A -> codegen B) wl wl' es x :
   run_codegen (c ≫= f) wl = inr (x, wl', es) ->
-  exists x1 wl1 es1 es2,
+  exists x1 wl1 wl2 es1 es2,
   run_codegen c wl = inr (x1, wl1, es1) /\
-  run_codegen (f x1) wl1 = inr (x, wl', es2) /\
+  run_codegen (f x1) (wl ++ wl1) = inr (x, wl2, es2) /\
+  wl' = wl1 ++ wl2 /\
   es = es1 ++ es2.
 Proof.
   intros H.
   rewrite run_codegen_def in H.
-  apply runWriterT_runStateT_sum_bind_dist in H.
-  destruct H as (x1 & s1 & l1 & l2 & H1 & H2 & H3).
-  exists x1, s1, l1, l2.
+  apply runWriterT_runAccumT_sum_bind_dist in H; [|by typeclasses eauto].
+  destruct H as (x1 & s1 & s2 & l1 & l2 & H1 & H2 & Hwl' & Hes).
+  exists x1, s1, s2, l1, l2.
   rewrite !run_codegen_def.
-  split.
+  split; [|split; [|split]].
   - assumption.
-  - split.
-    + assumption.
-    + unfold monoid_plus, Monoid_list_app in H3.
-      assumption.
+  - assumption.
+  - assumption.
+  - assumption.
 Qed.
 
 Lemma run_codegen_lift_error_inr {A} c wl wl' es (x : A) :
   run_codegen (lift_error c) wl = inr (x, wl', es) ->
-  c = inr x /\ wl' = wl /\ es = [].
+  c = inr x /\ wl' = [] /\ es = [].
 Proof.
   intros H.
   destruct c; cbn in H; first congruence.
@@ -194,35 +213,43 @@ Qed.
 
 Lemma run_codegen_try_option_inr {A} (c: option A) e x wl wl' es :
   run_codegen (try_option e c) wl = inr (x, wl', es) ->
-  c = Some x /\ wl' = wl /\ es = [].
+  c = Some x /\ wl' = [] /\ es = [].
 Proof.
   intros H.
   destruct c; cbn in H; [|congruence].
   inversion H; auto.
 Qed.
+  Check pass.
 
-Lemma run_codegen_capture {A} (c : codegen A) wl wl' es es' x :
+Lemma run_codegen_capture {A} (c : codegen A) (wl wl': wlocal_ctx) es es' x :
   run_codegen (capture c) wl = inr (x, es', wl', es) ->
   run_codegen c wl = inr (x, wl', es') /\ es = [].
 Proof.
   intros H.
+  unfold run_codegen.
+  unfold capture, censor, pass, listen, MonadWriter_codegen in H.
+  unfold listen in H.
+  cbn in H.
+  unfold pass in H.
+  cbn in H.
   unfold run_codegen in *.
   cbn in H.
-  destruct (runWriterT (runStateT (uncodegen c) wl)); first congruence.
+  destruct (runWriterT (runAccumT (uncodegen c) wl)); first congruence.
   cbn in H.
   destruct p.
   cbn in *.
   destruct pfst.
   cbn in H.
   inversion H.
-  subst a psnd l es.
+  subst a psnd wl' es.
   clear H.
+  rewrite app_nil_r.
   split; reflexivity.
 Qed.
 
 Lemma run_codegen_ret {A} (a: A) wl wl' x es :
   run_codegen (mret a) wl = inr (x, wl', es) ->
-  x = a /\ wl' = wl /\ es = [].
+  x = a /\ wl' = [] /\ es = [].
 Proof.
   intros Hret.
   inversion Hret.
@@ -232,7 +259,7 @@ Qed.
 Lemma run_codegen_emit wl e x wl' es' :
   run_codegen (emit e) wl = inr (x, wl', es') ->
   x = tt /\
-  wl' = wl /\
+  wl' = [] /\
   es' = [e].
 Proof.
   intros Hemit.
@@ -243,7 +270,7 @@ Qed.
 Lemma run_codegen_emit_all wl es x wl' es' :
   run_codegen (emit_all es) wl = inr (x, wl', es') ->
   x = tt /\
-  wl' = wl /\
+  wl' = [] /\
   es' = es.
 Proof.
   intros Hemit.
@@ -260,11 +287,12 @@ Ltac inv_cg_try_option Hrun :=
   destruct Hrun as (Heq1 & Heq2 & Heq3);
   rewrite ?Heq1, ?Heq2, ?Heq3 in *.
 
-Ltac inv_cg_bind Hbind res wl es1 es2 Hcg1 Hcg2 :=
+Ltac inv_cg_bind Hbind res wl1 wl2 es1 es2 Hcg1 Hcg2 :=
+  let Hwleq := fresh "Hwl_app_eq" in
   let Heseq := fresh "Hes_app_eq" in
   apply run_codegen_bind_dist in Hbind;
-  destruct Hbind as (res & wl & es1 & es2 & Hcg1 & Hcg2 & Heseq);
-  rewrite Heseq.
+  destruct Hbind as (res & wl1 & wl2 & es1 & es2 & Hcg1 & Hcg2 & Hwleq & Heseq);
+  rewrite Heseq, Hwleq.
 
 Ltac inv_cg_ret Hret :=
   let Hretval := fresh "Hretval" in
@@ -293,10 +321,10 @@ Ltac inv_cg_emit_all Hemit :=
 Example emit_ret_test wl x y z :
   run_codegen (emit W.BI_nop;;
                mret 7) wl = inr (x, y, z) ->
-  x = 7 /\ y = wl /\ z = [W.BI_nop].
+  x = 7 /\ y = [] /\ z = [W.BI_nop].
 Proof.
   intros Hrun.
-  inv_cg_bind Hrun res wl' es1 es2 Hemit Hret.
+  inv_cg_bind Hrun res wl1 wl2 es1 es2 Hemit Hret.
   inv_cg_emit Hemit.
   inv_cg_ret Hret.
   rewrite app_nil_r.
