theories/compiler/accum.v
@@ -1,0 +1,77 @@
+(* Accumulating state monad *)
+(* Like a state monad with S = list A, but writes append to the state
+   instead of replacing the state. *)
+
+From stdpp Require Import base.
+From ExtLib.Structures Require Import Functor Monads Monoid.
+
+Section Accum.
+  Variables 
+    (S : Type)
+    (m : Type -> Type).
+  
+  Record accumT (t: Type) : Type :=
+    mkAccumT { runAccumT : list S -> m (t * list S)%type }.
+  Arguments mkAccumT {t} _.
+  Arguments runAccumT {t} _.
+
+  Variable M : Monad m.
+
+  Definition evalAccumT {t} (c : accumT t) (s : list S) : m t :=
+    bind (runAccumT c s) (fun x => ret (fst x)).
+
+  Definition execAccumT {t} (c : accumT t) (s : list S) : m (list S) :=
+    bind (runAccumT c s) (fun x => ret (snd x)).
+
+  Global Instance Monad_accumT : Monad accumT :=
+  { ret := fun _ x => mkAccumT (fun s => @ret _ M _ (x, nil))
+  ; bind := fun _ _ c1 c2 =>
+    mkAccumT (fun s =>
+      @bind _ M _ _ (runAccumT c1 s)
+        (fun '(v, s') =>
+           @bind _ M _ _ (runAccumT (c2 v) (s ++ s')) 
+             (fun '(v, s'') => ret (v,s' ++ s''))))
+  }.
+
+  Global Instance MonadT_accumT : MonadT accumT m :=
+  { lift := fun _ c => mkAccumT (fun s => bind c (fun t => ret (t, nil)))
+  }.
+
+  Global Instance Exc_accumT T (MR : MonadExc T m) : MonadExc T accumT :=
+  { raise := fun _ e => lift (raise e)
+  ; catch := fun _ body hnd =>
+    mkAccumT (fun s => catch (runAccumT body s) (fun e => runAccumT (hnd e) s))
+  }.
+
+  Global Instance MonadZero_stateT (MR : MonadZero m) : MonadZero accumT :=
+  { mzero _A := lift mzero
+  }.
+
+  Global Instance MonadFix_stateT (MF : MonadFix m) : MonadFix accumT :=
+  { mfix := fun _ _ r v =>
+    mkAccumT (fun s => mfix2 _ (fun r v s => runAccumT (mkAccumT (r v)) s) v s)
+  }.
+
+  Global Instance MonadPlus_stateT (MP : MonadPlus m) : MonadPlus accumT :=
+  { mplus _A _B a b :=
+      mkAccumT (fun s => bind (mplus (runAccumT a s) (runAccumT b s))
+               (fun res => match res with
+                             | inl (a,s') => ret (inl a, s')
+                             | inr (b,s') => ret (inr b, s')
+                           end))
+  }.
+  
+  Global Instance MonadWriter_accumT T (Mon : Monoid T) (MR : MonadWriter Mon m) : MonadWriter Mon accumT :=
+  { tell := fun x => mkAccumT (fun s => bind (tell x) (fun v => ret (v, nil)))
+  ; listen := fun A (c: accumT A) =>
+                mkAccumT (fun s => bind (listen (runAccumT c s))
+                                         (fun x => let '(a,s',t) := x in ret (a,t,s')))
+  ; pass := fun _ c =>
+              mkAccumT (fun s => bind (runAccumT c s) 
+                                       (fun x => let '(a,t,s') := x in pass (ret ((a,s'),t))))
+  }.
+
+End Accum.
+
+Arguments mkAccumT {S m t} _.
+Arguments runAccumT {S m t} _.
